day01_2.v
@@ -4,19 +4,17 @@ From Coq Require Import
      extraction.ExtrOcamlIntConv.
 Import ListNotations.
 
-From SimpleIO Require Import
-     IOMonad CoqPervasives Utils.
+From SimpleIO Require
+     IOMonad CoqPervasives.
 
-Import IONotations.
+From ExtLib Require Import
+     Structures.Monads.
+Import MonadNotation.
+Local Open Scope monad.
+
+From advent Require Import lib.
 
 Module ZSet := FSetAVL.Make Z_as_OT.
-
-Definition read_Z : IO Z :=
-  map_io z_of_int read_int.
-
-Definition print_Z (z : Z) : IO unit :=
-  print_int (int_of_z z);;
-  print_newline.
 
 Definition cycle_aux {A} (self : Stream A) : list A -> Stream A :=
   cofix cycle_aux (xs : list A) : Stream A :=
@@ -31,13 +29,19 @@ Definition cycle {A} (xs : list A) : option (Stream A) :=
   | x :: xs => Some (cofix res := Cons x (cycle_aux res xs))
   end.
 
-Definition parse_stream : IO (Stream Z) :=
-  fix_io (fun loop acc =>
-    oz <- catch_eof read_Z;;
+Section main.
+
+Context {m : Type -> Type}
+        `{Monad m} `{MonadError m}
+        `{MonadIOZ m} `{MonadFix m}.
+
+Definition parse_stream : m (Stream Z) :=
+  mfix (fun loop acc =>
+    oz <- read_Z;;
     match oz with
     | None =>
       match cycle (rev acc) with
-      | None => prerr_endline "empty input";; exit_nat 1
+      | None => error "empty input"
       | Some s => ret s
       end
     | Some z => loop (z :: acc)
@@ -45,18 +49,22 @@ Definition parse_stream : IO (Stream Z) :=
 
 Definition no_seen : ZSet.t := ZSet.empty.
 
-Definition search (s : Stream Z) : IO Z :=
-  fix_io (fun loop '(seen, pos, (Cons z s)) =>
+Definition search (s : Stream Z) : m Z :=
+  mfix (fun loop '(seen, pos, (Cons z s)) =>
     if ZSet.mem pos seen then
       ret pos
     else
       loop (ZSet.add pos seen, (pos + z)%Z, s)
   ) (no_seen, 0%Z, s).
 
-Definition main : IO unit :=
+Definition main : m unit :=
   s <- parse_stream;;
   z <- search s;;
   print_Z z.
+
+End main.
+
+Import SimpleIO.IOMonad.
 
 Definition exec : io_unit := unsafe_run main.
 
