lib/io.v
@@ -1,0 +1,63 @@
+(* Interface for IO. *)
+
+From Coq Require Import
+     List ZArith String
+     extraction.ExtrOcamlIntConv.
+Import ListNotations.
+
+From Coq.extraction Require Import
+     ExtrOcamlIntConv.
+
+From ExtLib Require Import
+     Data.Monads.OptionMonad
+     Structures.Monads.
+
+From SimpleIO Require Import
+     IOMonad CoqPervasives Utils.
+
+Class MonadError (m : Type -> Type) : Type := {
+  error : forall a, string -> m a;
+}.
+
+Arguments error {m _ a}.
+
+Class MonadIOZ (m : Type -> Type) : Type := {
+  read_Z : m (option Z);
+  print_Z : Z -> m unit;
+}.
+
+(* Implementation *)
+
+Instance Monad_IO : Monad IO := {
+  Monad.ret := @IOMonad.ret;
+  Monad.bind := @IOMonad.bind;
+}.
+
+Instance MonadFix_IO : MonadFix IO := {
+  mfix := @fix_io;
+}.
+
+Module IO.
+
+Import IONotations.
+
+Definition error (a : Type) (s : string) : IO a :=
+  prerr_endline s;; exit_nat 1.
+
+Definition read_Z : IO (option Z) :=
+  catch_eof (map_io z_of_int read_int).
+
+Definition print_Z (z : Z) : IO unit :=
+  print_int (int_of_z z);;
+  print_newline.
+
+End IO.
+
+Instance MonadError_IO : MonadError IO := {
+  error := IO.error;
+}.
+
+Instance MonadIOZ_IO : MonadIOZ IO := {
+  read_Z := IO.read_Z;
+  print_Z := IO.print_Z;
+}.
