lib/mock.v
@@ -1,0 +1,80 @@
+(* Mocking the IO interface with pure functions. *)
+
+From Coq Require Import
+     List ZArith
+     extraction.ExtrOcamlIntConv.
+Import ListNotations.
+
+From Coq.extraction Require Import
+     ExtrOcamlIntConv.
+
+From ExtLib Require Import
+     Data.Monads.OptionMonad
+     Structures.Monads.
+
+From advent.lib Require Import
+     io.
+
+Definition input : Type := list Z.
+Definition output : Type := list Z.
+
+Record mock (r : Type) (a : Type) : Type := Mk_mock {
+  un_mock :
+    (a -> output -> input (* remaining *) -> r) ->
+    input ->
+    r;
+}.
+
+Arguments Mk_mock {r a} _.
+Arguments un_mock {r a} _.
+
+Global Instance Monad_mock r : Monad (mock r) := {
+  ret _ a := Mk_mock (fun k => k a []);
+  bind _ _ m k := Mk_mock (fun q =>
+    un_mock m (fun a o =>
+    un_mock (k a) (fun a o' =>
+    q a (o ++ o'))));
+}.
+
+Global Instance MonadIOZ_mock r : MonadIOZ (mock r) := {
+  read_Z := Mk_mock (fun k zs =>
+    match zs with
+    | [] => k None [] []
+    | z :: zs => k (Some z) [] zs
+    end);
+  print_Z z := Mk_mock (fun k zs => k tt [] [z]);
+}.
+
+(* Fuel for [mfix] *)
+Definition fuelT (m : Type -> Type) a :=
+  nat -> m (option a).
+
+Import MonadNotation.
+Local Open Scope monad_scope.
+
+Instance Monad_fuelT (m : Type -> Type)
+         `{Monad m} : Monad (fuelT m) := {
+  ret _ a := fun _ => Monad.ret (Some a);
+  bind _ _ m k := fun fuel =>
+    o <- m fuel;;
+    match o with
+    | None => Monad.ret None
+    | Some a => k a fuel
+    end;
+}.
+
+Instance MonadFix_fuelT (m : Type -> Type)
+         `{Monad m} : MonadFix (fuelT m) := {
+  mfix _ _ gf := fun a fuel0 =>
+    (fix go fuel a :=
+      match fuel with
+      | O => Monad.ret None
+      | S fuel' => gf (fun a _ => go fuel' a) a fuel0
+      end) fuel0 a
+}.
+
+Instance MonadIOZ_fuelT (m : Type -> Type)
+         `{Monad m} `{MonadIOZ m} : MonadIOZ (fuelT m) := {
+  read_Z := fun _ => liftM Some read_Z;
+  print_Z z := fun _ => liftM Some (print_Z z);
+}.
