lib/mock_spec.v
@@ -1,0 +1,188 @@
+(* Failed attempts at defining specifications on mocked programs.
+   Damn [mfix].
+ *)
+
+From Coq Require Import
+     List ZArith
+     extraction.ExtrOcamlIntConv.
+Import ListNotations.
+
+From Coq.extraction Require Import
+     ExtrOcamlIntConv.
+
+From ExtLib Require Import
+     Data.Monads.OptionMonad
+     Structures.Monads.
+
+From advent.lib Require Import
+     io mock.
+
+(* partial correctness *)
+Module fuel_partial.
+
+Definition spec' {a : Type}
+           (m : fuelT (mock Prop) a)
+           (i : input)
+           (post : input -> Prop) (o : output) (x : a) : Prop :=
+  forall fuel,
+    un_mock (m fuel) (fun ox' i' o' =>
+                        forall x', ox' = Some x' ->
+                                   x' = x /\
+                                   post i' /\
+                                   o' = o) i.
+
+Lemma spec_fix {a b} gf i (post : input -> Prop) o (x : a) (y : b) :
+  spec' (gf (mfix gf) x) i post o y ->
+  spec' (mfix gf x) i post o y.
+Proof.
+  intros Hspec fuel.
+Abort.
+
+End fuel_partial.
+
+Module fuel.
+
+Definition spec' {a : Type}
+           (m : fuelT (mock Prop) a)
+           (i : input)
+           (post : input -> Prop) (o : output) (x : a) : Prop :=
+  exists min_fuel,
+    forall (P : _ -> _ -> _ -> Prop) fuel,
+      fuel >= min_fuel ->
+      (forall x' i' o',
+          x' = Some x /\ post i' /\ o' = o -> P x' i' o') ->
+      un_mock (m fuel) P i.
+
+Definition spec (m : fuelT (mock Prop) unit) (i : input) (o : output) : Prop :=
+  exists min_fuel,
+    forall fuel,
+      fuel >= min_fuel ->
+      un_mock (m fuel) (fun x' i' o' =>
+                             x' = Some tt /\ o' = o) i.
+
+Lemma unfold_spec m i o :
+  spec' m i (fun _ => True) o tt ->
+  spec m i o.
+Proof.
+  intros [min_fuel Hspec'].
+  exists min_fuel.
+  intros fuel Hfuel.
+  apply Hspec'; auto.
+  firstorder.
+Qed.
+
+Lemma strong_post {a} m i (post1 post2 : input -> Prop) o (x : a) :
+  (forall i', post1 i' -> post2 i') ->
+  spec' m i post1 o x ->
+  spec' m i post2 o x.
+Proof.
+  intros Hpost [min_fuel Hspec'].
+  exists min_fuel. intros P fuel Hfuel HP.
+  apply Hspec'; auto.
+  firstorder.
+Qed.
+
+Lemma spec_fix {a b} gf i (post : input -> Prop) o (x : a) (y : b) :
+  spec' (gf (mfix gf) x) i post o y ->
+  spec' (mfix gf x) i post o y.
+Proof.
+  intros [min_fuel Hspec].
+  exists (S min_fuel); intros P fuel Hfuel HP.
+  induction fuel.
+  - inversion Hfuel.
+  - simpl.
+Abort.
+
+End fuel.
+
+(* Interpret the CPS-style [mock] as a predicate transformer. *)
+Module wp.
+
+Notation wp := (mock Prop).
+
+Definition incl_wp {a : Type} (m1 m2 : wp a) : Prop :=
+  forall q i, un_mock m1 q i -> un_mock m2 q i.
+
+Notation GF_wp a b := ((a -> wp b) -> (a -> wp b)).
+
+(*
+Definition mfix_wp {a b : Type}
+          (gf : GF_wp a b)
+          (x : a)
+          (q : b -> input -> output -> Prop)
+          (i : input) : Prop :=
+  forall
+    (P : a -> mock Prop b)
+    (P_ind : forall y, incl_wp (P y) (gf P y)),
+    un_mock (P x) q i.
+*)
+
+Variant mfix_wp {a b : Type}
+          (gf : GF_wp a b)
+          (x : a)
+          (q : b -> input -> output -> Prop)
+          (i : input) : Prop :=
+| MWP
+    (P : a -> mock Prop b)
+    (PHolds : un_mock (P x) q i)
+    (P_ind :forall y, incl_wp (P y) (gf P y))
+.
+
+Global Instance MonadFix_mock_Prop : MonadFix wp := {
+  mfix _ _ gf x := Mk_mock (mfix_wp gf x)
+}.
+
+Definition monotonic_wp {a b : Type}
+           (gf : GF_wp a b) :=
+  forall m1 m2,
+    (forall x, incl_wp (m1 x) (m2 x)) ->
+    (forall x, incl_wp (gf m1 x) (gf m2 x)).
+
+Theorem mfix_incl_1 {a b : Type}
+        (gf : GF_wp a b)
+        (gf_mon : monotonic_wp gf)
+        (x : a) :
+  incl_wp (mfix gf x) (gf (mfix gf) x).
+Proof.
+  intros q i [P PHolds P_ind]; simpl.
+  eapply gf_mon.
+  - unfold incl_wp; simpl.
+    intros.
+    econstructor.
+    + eauto.
+    + apply P_ind.
+  - apply P_ind; auto.
+Qed.
+
+(*
+Theorem mfix_incl_1 {a b : Type}
+        (gf : GF_mp a b)
+        (gf_mon : monotonic_mp gf)
+        (x : a) :
+  incl_mp (mfix gf x) (gf (mfix gf) x).
+Proof.
+  intros q i [P PHolds P_ind]; simpl.
+  eapply gf_mon.
+  - unfold incl_mp; simpl.
+    intros.
+    econstructor.
+    + eauto.
+    + apply P_ind.
+  - apply P_ind; auto.
+Qed.
+*)
+
+Theorem mfix_incl_2 {a b : Type}
+        (gf : GF_wp a b)
+        (gf_mon : monotonic_wp gf)
+        (x : a) :
+  incl_wp (gf (mfix gf) x) (mfix gf x).
+Proof.
+  intros q i H.
+  econstructor.
+  - eapply H.
+  - intros x' q' i'. intro.
+    eapply gf_mon; eauto.
+Abort.
+
+End wp.
