Makefile
@@ -1,3 +1,11 @@
-%.native: %.v
+.PHONY: lib
+
+lib: Makefile.coq
+	$(MAKE) -f Makefile.coq
+
+Makefile.coq: _CoqProject
+	coq_makefile -f _CoqProject -o $@
+
+%.native: lib %.v
 	coqc $(shell cat _CoqProject) $*.v
 	ocamlc $*.mli $*.ml -o $@
